iris/IregLinkNz.v
@@ -94,7 +94,7 @@ Section IregLinkNz.
     iDestruct (ireg_slots_acc_upd γi (ireg_bi inum) ds (islot inum) Hsl Hlen16
                 with "Hsls") as "[Hslot Hslback]".
     iEval (rewrite Hkey) in "Hslot".
-    iDestruct "Hslot" as "[(%wl & %gl & %rl & %cl & Hla & %Hlok & %Hrt) [Hep Harm]]".
+    iDestruct "Hslot" as "[(%wl & %wd & %gl & %rl & %cl & Hla & %Hlok & %Hrt & %Hdir) [Hep Harm]]".
     iDestruct (link_w_ge with "Hla Hfrag") as %Hw1.
     rewrite /dinode_at.
     iDestruct (ghost_map_lookup with "Ha Hdn") as %Hm.
@@ -116,7 +116,7 @@ Section IregLinkNz.
       iApply ("Hslback" $! (ds !!! islot inum) with "[Harm Hla Hep]").
       rewrite Hkey.
       iApply (ireg_slot_intro γi (bv_unsigned inum) (ds !!! islot inum)
-                wl gl cl rl Hlok Hrt with "Hla Hep"). iExact "Harm". }
+                wl wd gl cl rl Hlok Hrt Hdir with "Hla Hep"). iExact "Harm". }
     iModIntro. iFrame "Hdn Hfrag". iPureIntro. exact Hnz.
   Qed.
 
