iris/ProofSysLinkTails.v
@@ -1351,7 +1351,7 @@ Section ProofSysLinkTails.
                  ltac:(wp_next_chain) with "Hown") as "Hown".
     iApply (Iupdate.wp_iupdate_unlink (CID := CID8) gs jx gl gu gd gk pd pav pu
               bn g gfs gi cov logstart inodestart nib dev (ientry kk) inum
-              dn' dn bm u Sb true pidv dq (DfracOwn (1/2)) (DfracOwn (1/2)) dqs
+              dn' dn bm u Sb true None pidv dq (DfracOwn (1/2)) (DfracOwn (1/2)) dqs
               P4 (K - 38)%nat eb b lks
               HKiup ltac:(intros _; exact Hmem) Hgeom Hist0 Hiblk Hiblog Hinb
               ltac:(exact (sl_setnl_type_stable dn (sl_ndec (di_nlink dn))))
